CLean.lean
@@ -8,4 +8,5 @@ import CLean.Lemmas
 import CLean.Execution
 import CLean.PTXAst
 import CLean.PTXLowering
+import CLean.PTXParser
 import CLean.Examples
